## Sequences

$a_0,a_1,a_2,...$
We denote the sequence by $\{a_n\}_{n=0}^\infty$, $\{a_n\}_n$ or $\{a_n\}$

## Recurrence relations and initial conditions

_Recurrence relation_ for $a_n$ - relates $a_n$ to some of its predecessors
_Initial conditions_

A _closed form_ recurrence relation is a formula that solves $a_n$ in terms of $n$.

>__Example:__ the Fibonacci sequence: $$f_n = f_{n-1} + f_{n-2}\space ,\quad n \geq 3$$

A relation is __homogeneous__ if EVERY term requires one or more terms in the sequence: $$\mathnormal {Example:}\space a_n = a_{n-3}^3sin^2(a_{n-4}) + 7a_{n-2}^3$$
Otherwise, the relation is __inhomogeneous__: $$\mathnormal{Example:}\space a_n = a_{n-3}^3sin^2(a_{n-4}) + 7a_{n-2}^3 + \underline{7n + 4}$$
A recurrence relation is __linear homogeneous of order k with constant coefficients__ if it is of the form$$a_n = c_1a_{n-1}+c_2a_{n-2}+...+c_ka_{n-k}$$ 
>__Example:__ The recurrence relation $$a_n=3a_{n-1}-5a_{n-4}$$is linear homogeneous of order 4 with constant coefficients.

## General Solution for the Double Real Root Case

$$a_n = At_1^n + Bt_2^n$$

## General Solution for the Single Real Root Case

The general solution to $a_n = c_1 a_{n-1} + c_2 a_{n-2}$ for the case when the associated characteristic equation $t^2 - c_1 t - c_2 = 0$ has a unique real solution $t = r$, is of the form $$a_n = Ar^n + Bnr^n.$$
## General solution for double real root case
The general solution to $$a_n = c_1 a_{n-1} + c_2 a_{n-2}$$ for the case when the associated characteristic equation $$t^2 - c_1 t - c_2 = 0$$ has two distinct real solutions $t = t_1$ and $t = t_2$, of the form $$a_n = At_1^n + Bt_2^n$$
## Choice of the particular solution $p_n$
For the inhomogeneous recurrence relations $$a_n = c_1 a_{n-1} + c_2 a_{n-2} + f(n)$$
where $f(n)$ involves $cos(n)$ or $sin(n)$. In this case $p_n = a cos n +$

>__Example:__ Population growth
>
>Initial population $a_0$ = 1000
>$a_n = a_{n-1} + (0.1)a_{n-1} = (1.1)a_{n-1}$
>
>Which leads to $$\begin{gather}
a_n = (1.1)a_{n-1} \\
a_0 = 1000
\end{gather}$$ We can solve by _iteration_: $$\begin{align}
a_n &= 1.1 a_{n-1}\\
&= 1.1(1.1a_{n-2}) = (1.1)^2 a_{n-2}
\end{align}$$