Solve a problem with a function that calls itself

>Example:
>Calculate $n!$
>$3! = 3×2×1$
>$4! = 4 × (3×2×1)$
>So, $n! = n × Factorial(n-1)$

Steps:
1. Solve _simple case_ of a problem
2. Figure out how the _general_ case can be solved using the _simple case_

>Example:
>$Factorial(1) = 1$
>$Factorial(n) = n×(n-1)×(n-2)×...×1$
>$Factorial(n) = n × Factorial(n-1)$
>
>For example: 
>$\begin{align} Fact(3) &= 3 × Fact(2)\\ Fact(2) &= 2 × Fact(1)\\ Fact(1) &= 1 \end{align}$
>Then go back up:
>$\begin{align} Fact(2) &= 2×1 = 2\\ Fact(3) &= 3×2 = 6 \end{align}$

Using Lambda Calculus:
$\begin{align} (\lambda n.\ &if(=\ n\ 1)\\ &1\\ &(*\ n\ (fact (-\ n\ 1)))\ ) \end{align}$
