## 1.
---
$$f(x) = x - ln(x) - \sqrt 2$$
__(a)__
$$\begin{split}
x = 0.5,\quad &f(0.5) = 0.5 - ln(0.5) - \sqrt2 = -0.22666 \\
x = 1, \quad &f(1) = 1 - ln(1) - \sqrt2 = -0.414214 \\
... \\
x = 2.5, \quad &f(2.5) = 2.5 - ln(2.5) - \sqrt2 = 0.169469 \\
x = 3, \quad &f(3) = 3 - ln(3) - \sqrt2 = 
\end{split}$$
__(b)__
$$\begin{gather*}
&[a, b] = [2, 3] \\
&f(a) = -0.107361 \quad ; \quad f(b) = 0.487174 \\
&d = {2 + 3 \over 2} = {5 \over 2} = 2.5
\end{gather*}$$

| iteration |        $[a,b]$        | $a + b \over 2$ |   $f(a)$   |  $f(d)$   | $f(a)f(d)$ |
| :-------: | :-------------------: | :-------------: | :--------: | :-------: | :--------: |
|    $1$    |       $[2, 3]$        |      $2.5$      | $-0.1074$  | $0.1695$  |  $\lt 0$   |
|    $2$    |      $[2, 2.5]$       |     $2.25$      | $-0.1074$  | $-0.0429$ |  $\gt 0$   |
|    ...    |          ...          |       ...       |    ...     |    ...    |    ...     |
|     7     | $[2.203125, 2.21875]$ |   $2.2109375$   | $-0.00096$ | $-0.0033$ |  $\lt 0$   |
So, the estimation of the root is $2.2109375$.

## 3.
---
$$
\begin{gather*}
f(x) = e^{x + 2} - x^2 + 3x = 0 \\
f'(x) = e^{x + 2} - 2x + 3
\end{gather*}$$
Newton-Raphson:
$$\begin{gather*}
&&x_{n+1} = x_n - {f(x_n) \over f'(x_n)} = x_n - {e^{x_n + 2} - x_n^2 + 3x_n \over e^{x_n + 2} - 2x_n + 3} \\
&n = 0: &x_1 = ... = -0.7112345 \\
&n = 1: &x_2 = ... = -0.83404 \\
&n = 2: &x_3 = ... = -0.8354 \\
&n = 4: &x_4 = ... = 
\end{gather*}$$