## 1.
---

$$\begin{gather*}
&\text{Base case: } &sum(1) = 1\\
&\text{Inductive step: } &\text{Assume that } sum(k), k\in \mathbb{N}\\
&&\text{we define } sum(k+1) = sum(k) + (k+1)
\end{gather*}$$
## 2.
---
```java
int sum(int n, int result) {
	if (n == 1)
		return 1;
	return sum(n - 1, result + n);
}
```

## 3.
---
```java
int sum(int n) {
	int result = 0;
	for(int k = 1; k <= n; ++k)
		result += k;
	return result;
}
```

## 4.
---
$$
\begin{split}
	&\begin{gather*}
		&\text{Base case: } &2, 3, 4, ...\\
		&&\text{for any expression } value \geq 2\\
		&\text{Industive step: }
	\end{gather*}\\
	&\text{Assume that the value of an E-expression with k atomic expressions is at least }2k.\\
	&\text{We want to prove that the value of an expression formed from two expression}\\
	&\text{is at least } 2(k+1):\\
	&\text{The value of } (x + y) \text{ is at least } 2k + 2k = 4k \\
	&\text{The value of } (x * y) \text{ is at least } 2k * 2k = 4k^2 \\
	&\text{So, the value of any E-expression with } n \text{ atomic expressions is at least } 2n.
\end{split}$$

## 5.
---
$$
\begin{split}
&\begin{gather*}
	\text{Base case: } &n = 1 \Rightarrow m \text{ children}\\
	\text{Inductive step: } &\text{Assume that } n = k \Rightarrow m^{k-1}\\
							&\text{Next level has } m^{k-1} \text{ nodes}\\
							&\text{Each of them has } m \text{ children}\\
							&\text{So for } n = k+1 \text{ there are }\\
							&m^{k-1} \times m = m^k = m^{(k+1)-1} \text{ leaf nodes}\\
\end{gather*}\\
&\text{So an m-ary tree of height } n \text{ can have } m^{n-1} \text{ leaves}
\end{split}
$$
